\textbf{Problem 9}

\begin{solution}\ 
We have that 
\[\mathbb{E}[Y] = \sum_{y} yP(Y = y)\]
and that 
\[\mathbb{E}[Y|X] = \sum_y yP(Y = y | X)\]
%$$\mathbb{E}[Y|X] = \sum_{\omega} Y(\omega)p(\omega | X) = \sum_{\omega}i_{\omega}P(Y = i_{\omega} | X)$$
and we want to show that $\mathbb{E}[\mathbb{E}[Y|X]] = \mathbb{E}[Y]$.\\
Proceeding, we can see that 
$$\mathbb{E}[\mathbb{E}[Y|X]] = \sum_x \mathbb{E}[Y | X = x]P(X = y=x)$$

So, 
$$\sum_x \mathbb{E}[Y | X = x]P(X = x) = \sum_x \bigg(\sum_y yP(Y = y | X =x)\bigg)P(X = x)$$
$$\sum_x \mathbb{E}[Y | X = x]P(X = x) = \sum_x \bigg(\sum_y y\frac{P(Y = y \text{ and } X =x)}{P(X =x )}\bigg)P(X = x)$$

$$\sum_x \mathbb{E}[Y | X = x]P(X = x) = \sum_x \bigg(\sum_y y\frac{P(Y = y \text{ and } X =x)}{P(X =x )}\bigg)P(X = x)$$
$$\sum_x \mathbb{E}[Y | X = x]P(X = x) = \sum_x \sum_y yP(Y = y \text{ and } X =x)$$
$$\sum_x \mathbb{E}[Y | X = x]P(X = x) = \sum_y y\bigg(\sum_x P(Y = y \text{ and } X =x)\bigg)$$

$$\sum_x \mathbb{E}[Y | X = x]P(X = x) = \sum_y yP(Y = y)$$
which is that 
\[\mathbb{E}[\mathbb{E}[Y|X]] = \mathbb{E}[Y]\]


%$$\mathbb{E}[\mathbb{E}[Y|X]] = \mathbb{E}\bigg[\sum_{\omega} Y(\omega)p(\omega | X)\bigg]$$
%$$\mathbb{E}[\mathbb{E}[Y|X]] = \mathbb{E}\bigg[\sum_y yP(Y = y | X)\bigg]$$

%$$\mathbb{E}[\mathbb{E}[Y|X]] = \sum_xx\bigg(\sum_y yP(Y = y | X =x )\bigg)P(X = x)$$

%\begin{align}
%\mathcal{L}^{-1}\left\{f(d)\right\} &= \mathcal{L}^{-1}\left\{f_1(\delta).f_2(\delta)\right\} \\
%& = \exp(mt) \star \left\{\frac{l}{2\sqrt{\pi t^3}} \exp(-l^2/{4t})\right\} \\
%& = F_1 * F_2
%\end{align}

\end{solution}

\textbf{We affirm that we have adhered to the Honor Code in this assignment.}