\textbf{Problem 7}

\begin{solution}\ 

%NOTE: some facts
%\[\text{E}[Y] = \int_0^1yp_Ydy\]
%\[B(\alpha, \beta) = \frac{(\alpha - 1)!(\beta - 1)!}{(\alpha + \beta - 1)!}\]
%\[B(\alpha, \beta, y) = \frac{1}{B(\alpha, \beta)}y^{\alpha -1}(1-y)^{\beta -1}\]
%\[B(\alpha, \beta) = \frac{\Gamma(\alpha)\Gamma(\beta)}{\Gamma(\alpha + \beta)}\]
%\[\frac{\Gamma(\alpha)\Gamma(\beta)}{\Gamma(\alpha + \beta)} = \int_0^1 y^{\alpha-1}(1-y)^{\beta-1}dy \]
%\[\Gamma(x+1) = x\Gamma(x)\]

The probability density function of random variable $Y$ with the beta distribution on the interval $[0,1]$ is given here:
\[p_Y(y) = \frac{\Gamma(\alpha + \beta)}{\Gamma(\alpha)\Gamma(\beta)}y^{\alpha -1}(1-y)^{\beta -1}\]
We proceed to find the expected value of $Y$:
\[\mathbb{E}[Y] = \int_0^1yp_Ydy\]
\[\mathbb{E}[Y] = \int_0^1y\frac{\Gamma(\alpha + \beta)}{\Gamma(\alpha)\Gamma(\beta)}y^{\alpha -1}(1-y)^{\beta -1} dy\]
\[\mathbb{E}[Y] = \frac{\Gamma(\alpha + \beta)}{\Gamma(\alpha)\Gamma(\beta)}\int_0^1yy^{\alpha -1}(1-y)^{\beta -1} dy\]
\[\mathbb{E}[Y] = \frac{\Gamma(\alpha + \beta)}{\Gamma(\alpha)\Gamma(\beta)}\int_0^1y^{\alpha }(1-y)^{\beta -1} dy\]
\[\mathbb{E}[Y] = \frac{\Gamma(\alpha + \beta)}{\Gamma(\alpha)\Gamma(\beta)}\cdot\frac{\Gamma(\alpha + 1)\Gamma(\beta)}{\Gamma(\alpha + 1 + \beta)}\]
\[\mathbb{E}[Y] = \frac{\Gamma(\alpha + \beta)\Gamma(\alpha + 1)\Gamma(\beta)}
{\Gamma(\alpha)\Gamma(\beta)\Gamma(\alpha + 1 + \beta)}\]
\[\mathbb{E}[Y] = \frac{\Gamma(\alpha + \beta)\Gamma(\alpha + 1)}{\Gamma(\alpha)\Gamma(\alpha + 1 + \beta)}\]
\[\mathbb{E}[Y] = \frac{\Gamma(\alpha + \beta)\alpha\Gamma(\alpha )}{\Gamma(\alpha)
(\alpha + \beta)\Gamma(\alpha + \beta)}\]
\[\mathbb{E}[Y] = \frac{\alpha}{
\alpha + \beta}\]
\end{solution}